List_Ops.thy
@@ -19,25 +19,25 @@ next
     with Cons.prems show ?case by simp
   next
     assume "term \<noteq> x"
-    moreover with Cons.prems obtain idx' where "find_idx term xs = Some idx'" by fastforce
-    ultimately show ?case using Cons by fastforce
+    moreover with Cons.prems obtain idx' where "find_idx term xs = Some idx'" by force
+    ultimately show ?case using Cons by force
   qed
 qed
 
-lemma find_idx_Some:"term\<in>set xs \<longleftrightarrow> find_idx term xs \<noteq> None"
+lemma find_idx_Some:"term \<in> set xs \<longleftrightarrow> find_idx term xs \<noteq> None"
 proof
   have "term \<notin> set xs \<Longrightarrow> find_idx term xs = None"
     apply (induction xs)
-    by (auto)
-  thus "find_idx term xs \<noteq> None \<Longrightarrow> term\<in>set xs" by meson
+    by auto
+  thus "find_idx term xs \<noteq> None \<Longrightarrow> term \<in> set xs" by meson
 next
-  show "term\<in>set xs \<Longrightarrow> find_idx term xs \<noteq> None"
+  show "term \<in> set xs \<Longrightarrow> find_idx term xs \<noteq> None"
     apply (induction xs)
      apply simp
     by force
 qed
 
-lemma find_idx_None:"find_idx term xs = None \<longleftrightarrow> term\<notin> set xs" using find_idx_Some by metis 
+lemma find_idx_None:"find_idx term xs = None \<longleftrightarrow> term \<notin> set xs" using find_idx_Some by metis 
 
 lemma find_idx_Some_is_first:"\<lbrakk>find_idx term xs = Some idx; idx' < idx\<rbrakk> \<Longrightarrow> xs!idx' \<noteq> term"
 proof (induction xs arbitrary:idx idx')
@@ -48,13 +48,11 @@ next
   show ?case
   proof cases
     assume "term = x"
-    hence "idx = 0" using Cons.prems(1) by simp
-    hence False using Cons.prems(2) by simp
-    thus ?case by simp
+    thus ?case using Cons.prems by simp
   next
     assume "term \<noteq> x"
-    moreover with Cons.prems(1) obtain idx_1 where idx_1:"find_idx term xs = Some idx_1" using find_idx.simps by fastforce
-    ultimately have "idx = Suc idx_1" using find_idx.simps Cons.prems(1) by fastforce
+    moreover with Cons.prems(1) obtain idx_1 where idx_1:"find_idx term xs = Some idx_1" by fastforce
+    ultimately have "idx = Suc idx_1" using Cons.prems(1) by fastforce
     show ?case
     proof (cases idx')
       case 0
@@ -77,20 +75,14 @@ next
   show ?case
   proof (cases idx)
     case 0
-    with Cons.prems(3) have "term = x" by simp
-    thus ?thesis using 0 by simp
+    with Cons.prems(3) show ?thesis by force
   next
     case (Suc idx_1)
-    with Cons.prems(2) have "\<forall>idx'<idx_1. xs!idx' \<noteq> term" by (metis add_Suc_shift less_Suc_eq_le less_natE nat_arith.suc1 nat_le_iff_add nth_Cons_Suc)
-    moreover from Suc Cons.prems(1) have "idx_1 < length xs" by simp
-    moreover from Suc Cons.prems(3) have "xs!idx_1 = term" by simp
-    ultimately have "find_idx term xs = Some idx_1" using Cons.IH by simp
-    moreover from Cons.prems(2) Suc have "term \<noteq> x" by auto
-    ultimately show ?thesis using Suc by simp
+    thus ?thesis using Cons by fastforce
   qed
 qed
 
-lemma find_idx:"term\<in>set xs \<Longrightarrow> xs!the(find_idx term xs) = term"
+lemma find_idx:"term \<in> set xs \<Longrightarrow> xs!the(find_idx term xs) = term"
 proof (induction xs)
   case Nil
   thus ?case by simp
@@ -102,7 +94,7 @@ next
     thus ?case by simp
   next
     assume "term \<noteq> x"
-    with Cons.prems have prem:"term\<in>set xs" by auto
+    with Cons.prems have prem:"term \<in> set xs" by auto
     with find_idx_Some have "find_idx term xs \<noteq> None" by metis
     then obtain idx where idx:"find_idx term xs = Some idx" by blast
     hence "xs!idx = term" using Cons.IH prem by simp
